Vegas/Compile.lean
@@ -7,6 +7,7 @@ Authors: VegasCore contributors
 import Vegas.Compile.Compiler
 import Vegas.Compile.ConditionalExecution
 import Vegas.Compile.ConditionalOpeningSite
+import Vegas.Compile.ConditionalOpeningController
 import Vegas.Compile.ConditionalPublication
 import Vegas.Compile.ConditionalResolution
 import Vegas.Compile.PublicChoice
